\documentclass[20pt, letterpaper, titlepage]{article}
\usepackage[left=3.5cm, right=2.5cm, top=2.5cm, bottom=2.5cm]{geometry}
\usepackage[MeX]{polski}
\usepackage[utf8]{inputenc}
\usepackage{graphicx}
\usepackage{enumerate}
\usepackage{amsmath} %pakiet matematyczny
\usepackage{amssymb} %pakiet dodatkowych symboli
\usepackage{caption}
\captionsetup[table]{labelformat=empty}
\title{Pierwszy dokument LaTeX}
\begin{document}

\section{Wzory matematyczne}
\begin{LARGE}
$$ \sqrt{ \frac{2^{n}}{2_n}} \neq \sqrt[\frac{1}{3}]{1+n} $$

$$ \frac{2^k}{2^{k+2}} $$


$$ \frac{x^2}{2^{(x+2)(x-2)^3}} $$

$$ \log_22^{8} = 8$$

$$ \sqrt[3]{e^x - log_2x} $$

$$\lim_{x \to \infty } \sum_{k=1}^{n} \frac{1}{k^2} = \frac{\pi^2}{6}$$ 

$$\int_{2}^{\infty} \frac{1}{\log_2x}dx = \frac{1}{x} \sin x = 1 - \cos^2(x)$$

$$ \left[ \begin{array}{cccc}
a_{11} & a_{12} & \ldots & a_{1K} \\
a_{21} & a_{22} & \ldots & a_{2K}\\
\vdots & \vdots & \ddots & \vdots \\
a_{K1} & a_{K2} & \ldots & a_{KK}\\
\end{array} \right]*
\left[ \begin{array}{c}
x_{1} \\
x_{2} \\
\vdots \\
x_{K} \\
\end{array} \right]=
\left[ \begin{array}{c}
b_{1} \\
b_{2} \\
\vdots \\
b_{K} \\
\end{array} \right]$$

$$
(a_1 = a_1(x)) \wedge (a_2 = a_2(x)) \wedge \ldots \wedge (a_k = a_k(x)) \Rightarrow (d = d(u))
$$\\

$$
[x]_A = \{y \in U : a(x) = a(y),\forall a \in A\}, \text{where the control object} x \in U
$$\\

$$
T : [0,1] \times [0,1] \longrightarrow [0,1]
$$\\

$$
\lim_{x \to \infty} exp(-x) = 0
$$\\

$$
\frac{n!}{k!(n - k)!} = {n \choose k}\qquad
$$\\

$$
P{\left( A = 2 \bigg| \frac{A^2}{B} > 4 \right)}
$$\\


$$ S^{C_i}(a) = \frac{(\bar{C}_i^a) - \hat{C}_i^a)^2}{Z_{\bar{C}_i^{a^2}} + Z_{\hat{C}^{a^2}_i }}, a \in A $$\\

$$
\begin{cases}
|z| = |z - 4i| \\
\frac{\pi}{4} \geq Arg z < \frac{\pi}{2}\\
\end{cases}
$$\\

$$
\begin{cases}
|z + 4| = |z + 2 - 2i|\\
|z| \geq 2\\
\end{cases}
$$\\

$$
\begin{cases}
|z - 1 - i| < \sqrt{2}\\
Arg(z - 1 - i) < \frac{\pi}{2}\\
\end{cases}
$$\\

$$
\left\{
\begin{array}{rrrrr}
x & + & 5y & = & 2 \\
-3x & + & 6y & = & 15\\
\end{array}
\right.
$$\\

$$
\left\{
\begin{array}{rrrrrrr}
x & - & y & - & z & = & 1\\
3x & + & 4y & - & 2z & = & -1\\
3x & - & 2y & - & 2z & = & 1\\
\end{array}
\right.
$$\\

$$
\left\{
\begin{array}{rrrrrrrrr}
  &   & y & - & 3z & + & 4v & = & 0\\
x &  &  & - & 2z &  &  & = & 0\\
3x & + & 2y &   &   & - & 5v & = & 2\\
4x &  &  & - & 5z &  &  & = & 0\\
\end{array}
\right.
$$\\

$$
\begin{bmatrix}
1 & 0 & 0\\
0 & 3 & 0\\
0 & 0 & 1\\
\end{bmatrix}
*
\begin{bmatrix}
1 & 2 & 3\\
3 & 1 & 2\\
5 & 1 & 3\\
\end{bmatrix}
$$\\

$$
\left[ \begin{array}{rrr}
0 & 1 & 0\\
1 & 0 & 0\\
0 & 0 & 1\\
\end{array} \right]
*
\left[ \begin{array}{rr}
11 & -2\\
6 & -14\\
-21 & 30\\
\end{array} \right]
$$\\

$$
\left[ \begin{array}{rrr}
1 & 0 & 0\\
0 & 1 & 0\\
1 & 0 & 1\\
\end{array} \right]
*
\left[ \begin{array}{rrr}
1 & 1 & 3\\
2 & 1 & 4\\
1 & 3 & 0\\
\end{array} \right]
$$\\

$$
\left| \begin{array}{rr}
-3 & 2\\
8 & -5\\
\end{array} \right|
$$\\

$$
\left| \begin{array}{rr}
\sin \alpha & \cos  \alpha\\
\sin \beta & \cos \beta\\
\end{array} \right|
$$\\

$$
\left| \begin{array}{ccc}
1 & i & 1 + i\\
-i & 1 & 0\\
1 - i & 0 & 1\\
\end{array} \right|
$$\\

$$
\left[ \begin{array}{c|cc|ccc}
1 & 0 & 0 & 1 & 1 & 1\\ \hline
0 & 2 & 2 & 1 & 2 & 3\\
0 & 2 & 2 & 4 & 5 & 6\\ \hline
0 & 0 & 0 & 3 & 3 & 1\\
0 & 0 & 0 & 3 & 1 & 3\\
0 & 0 & 0 & 1 & 3 & 3\\
\end{array} \right]
$$\\

$$
\int_{1}^\infty \frac{dx}{(x+ 2)^2}
$$\\

$$
\int_{-\infty}^\infty \frac{dx}{x^2 + 4}
$$\\

$$
\int_{-\infty}^\infty x^2 exp^{{-x}^3} dx
$$\\

$$
\int_{1}^\infty \frac{dx}{\sqrt[3]{3x + 5}} 
$$\\

$$
\log_{\sqrt[3]{5}} 5\sqrt[3]{5}
$$\\

$$
\log_{\sqrt[3]{3}} 27
$$\\

$$
\log_2 \sqrt{2}
$$\\

$$
\lim_{n\to\infty} \left( \sqrt{n + 6 \sqrt{n} + 1}- \sqrt{n} \right)$$\\
$$
\lim_{n\to\infty}  \frac{{1 + \frac{1}{2}} + \frac{1}{2^2} + \ldots + \frac{1}{2^n}} {1 + \frac{1}{3} + \frac{1}{3^2} + \ldots + \frac{1}{3^n}}$$\\

$$
\sum_{n = 1}^\infty (-1)^{n+1} (2n -1) 
$$\\

$$
\sum_{n = 1}^\infty \sin \frac{2\pi}{3^n} \cos \frac{3\pi}{3^n}
$$\\

$$
\left[ \begin{array}{ccc}
1 & 2 & 3\\
0 & -6 & 7\\
\end{array} \right]^T
=
\left[ \begin{array}{cc}
1 & 0\\
2 & -6\\
3 & 7\\
\end{array} \right]
$$\\

$$
U_{AB} = \frac{W_{A \rightarrow B}}{q} = \int_A^B \vec{E} * \vec{dl}
$$\\
\end{LARGE}
\end{document}